Systems/States.v
@@ -1,5 +1,5 @@
 From mathcomp.ssreflect
-Require Import ssreflect ssrbool ssrnat eqtype ssrfun seq.
+Require Import ssreflect ssrbool ssrnat eqtype ssrfun seq fintype.
 From mathcomp
 Require Import path.
 Require Import Eqdep Relations.
@@ -11,60 +11,44 @@ Set Implicit Arguments.
 Unset Strict Implicit.
 Unset Printing Implicit Defensive.
 
-Section States.
-
-(* Number of nodes *)
-Variable N : nat.
+Definition Address_ordMixin := fin_ordMixin Address.
+Canonical Structure Address_ordType := OrdType Address Address_ordMixin.
 
 Definition StateMap := union_map [ordType of Address] State.
 
-Fixpoint initState' n : StateMap :=
-  if n is n'.+1 then (n \\-> Init n) \+ (initState' n') else Unit.
+Definition initState' s : StateMap := foldr (fun a m => (a \\-> Init a) \+ m) Unit s.
 
 (* Master-lemma, proving a conjunction of two mutually-necessary facts *)
-Lemma initStateValidDom n : dom (initState' n) =i iota 1 n /\ valid (initState' n).
+Lemma initStateValidDom s :
+  uniq s -> dom (initState' s) =i s /\ valid (initState' s).
 Proof.
-elim: n=>/=[|n [H1 H2]]; first by rewrite valid_unit dom0.
+elim: s => /=[|a s']; first by rewrite valid_unit dom0.
+move => IH.
+move/andP => [H_ni H_u].
+move/IH: H_u => [H1 H2] {IH}.
 split; last first.
-- case: validUn; rewrite ?um_validPt ?H2//. 
+- case: validUn; rewrite ?um_validPt ?H2//.
   move=>k; rewrite um_domPt inE=>/eqP Z; subst k.
-  by rewrite H1 mem_iota=>/andP[_]; rewrite add1n ltnn. 
-move=>z; rewrite domUn !inE !um_domPt !inE.
-case B: (z == 1)=>//=.
-- move/eqP: B=>B; subst z=>/=; apply/andP; split; last first.
-  + by rewrite orbC H1 mem_iota/= addnC addn1; case: n {H1 H2}=>//.
-  case: validUn; rewrite ?um_validPt ?H2//. 
-  move=>k; rewrite um_domPt inE=>/eqP Z; subst k.
-  by rewrite H1 mem_iota=>/andP[_]; rewrite add1n ltnn. 
-case C: (z \in iota 2 n).
-- apply/andP; split; last first.
-  + rewrite orbC H1 mem_iota/= addnC addn1; rewrite mem_iota in C.
-    case/andP: C=>H3 H4; rewrite eq_sym.
-    rewrite addnC addn2 in H4; clear B.
-    case B: (z == n.+1); rewrite orbC//=.
-    rewrite ltnS leq_eqVlt B/= in H4.
-    by rewrite H4 andbC/=; by case: {B H4} z H3.
-  case: validUn; rewrite ?um_validPt ?H2//. 
-  move=>k; rewrite um_domPt inE=>/eqP Z; subst k. 
-  by rewrite H1 mem_iota=>/andP[_]; rewrite add1n ltnn. 
-rewrite H1; apply/negP=>/andP[_]/orP[].
-- move/eqP=>Z; subst z; rewrite mem_iota in C.
-  move/negP: C=>C; apply: C; rewrite addnC addn2.
-  rewrite andbC ltnSn/=; clear H1 H2.
-  by move/negbT: B; case: n.
-rewrite !mem_iota in C *=>/andP[]H3 H4.
-move/negP: C=>C; apply: C; apply/andP; split.
-- by clear H4; case: z H3 B=>//z _; case: z=>//.
-rewrite addnC addn1 in H4; rewrite addnC.
-by rewrite addn2 -[n.+2]addn1; apply: ltn_addr. 
+  rewrite H1.
+  by move/negP: H_ni.
+- move=>z; rewrite domUn !inE !um_domPt !inE.
+  rewrite H1.
+  case validUn.
+  * by move/negP => H_v; case: H_v; rewrite um_validPt.
+  * by move/negP.
+  * move => k.
+    rewrite H1.
+    rewrite um_domPt inE=>/eqP H_eq.
+    rewrite -H_eq => H_in.
+    by move/negP: H_ni.
+  * move => Hv1 Hv2 H_d.
+    by rewrite eq_sym.
 Qed.
 
-Lemma valid_initState n : valid (initState' n).
-Proof. by case: (initStateValidDom n). Qed.
+Lemma valid_initState' s : uniq s -> valid (initState' s).
+Proof. by move => H_u; case: (initStateValidDom H_u). Qed.
 
-Lemma dom_initState n : dom (initState' n) =i iota 1 n.
-Proof. by case: (initStateValidDom n). Qed.
+Lemma dom_initState' s : uniq s -> dom (initState' s) =i s.
+Proof. by move => H_u; case: (initStateValidDom H_u). Qed.
 
-Definition initState := initState' N.
-
-End States.
+Definition initState := initState' (enum Address).
